tests/lean/SepLogic/Partial.lean
@@ -99,7 +99,7 @@ example (p : Ptr Nat) (Q : IPost Nat) : ¬ dispec emp (read p) Q := by
   intro hTriple
   rw [dispec_iff] at hTriple
   have hSpec := hTriple emp ∅ ((sep_emp_r emp).mpr ∅ trivial)
-  simp only [read, Result.guardedModify] at hSpec
+  simp only [Aeneas.Std.RawPtr.read, Result.guardedModify] at hSpec
   obtain ⟨hReadable, -⟩ := hSpec.vis_view
   exact Ptr.not_contains_empty p hReadable.contains
 
